beginning to convert to gmap (done until Patterns.v)

theories/Block.v
@@ -2,69 +2,45 @@
     and proves the correctness and completeness of that function. *)
 
 From Vellvm Require Import Syntax ScopeTheory Semantics.
-From ITree Require Import ITree Eq.
-Require Import FSets.FMapAVL FSets.FMapFacts.
+(* From ITree Require Import ITree Eq. *)
+(* Require Import FSets.FMapAVL FSets.FMapFacts. *)
 Require Import List.
-Import ListNotations.
-From Pattern Require Import IdModule MapCFG.
-Import Map MapF MapF.P MapF.P.F.
-Import IdOT MapCFG.
+Import gmap.
+(* Import ListNotations. *)
+From Pattern Require Import Base.
+(* Import Map MapF MapF.P MapF.P.F. *)
+(* Import IdOT MapCFG. *)
 
-Definition blocks_aux (G: map_cfg) : _ -> (blk*map_cfg) := fun '(id, b) => (b, remove id G).
+Definition blocks_aux (G: ocfg) : (bid*blk) -> (bid*blk*ocfg) := fun '(id, b) => (id, b, delete id G).
 
-Definition blocks (G: map_cfg): list (blk*map_cfg) := List.map (blocks_aux G) (elements G).
+Definition blocks (G: ocfg): list (bid*blk*ocfg) := map (blocks_aux G) (map_to_list G).
 
-Record blocks_aux_sem (G0 G G': map_cfg) b : Prop := 
+Record blocks_aux_sem (G0 G G': ocfg) id b : Prop := 
   {
-    MT: MapsTo_id b G;
-    RM: G' = remove_id b G0;
-    WF: wf_map_cfg G'
+    EQ: G' = delete id G0;
+    IN: G !! id = Some b
   }.
 
-Definition blocks_sem (G G': map_cfg) b := blocks_aux_sem G G G' b.
+Definition blocks_sem (G G': ocfg) id b := blocks_aux_sem G G G' id b.
 
-Definition P G0 G := forall G' b, wf_map_cfg G -> wf_map_cfg G0 ->
-  ((b, G') ∈ (List.map (blocks_aux G0) (elements G))) <-> blocks_aux_sem G0 G G' b.
+Definition blocks_aux_P G := forall G0 G' id b, 
+  ((id, b, G') ∈ (map (blocks_aux G0) (map_to_list G))) <-> blocks_aux_sem G0 G G' id b.
 
-Lemma blocks_aux_correct: forall G0 G, P G0 G.
+Lemma blocks_aux_correct: forall G, blocks_aux_P G.
 Proof.
-  intros G0 G.
-  apply map_induction_min; unfold P.
-  - intros E Em G' B WFE WF0. split.
-    * assert (Enil: elements E = []) by now apply elements_Empty. now rewrite Enil.
-    * intros [MTE _ _]. contradict MTE. intro MTE. eapply empty_mapsto_iff.
-      eapply MapsTo_m. reflexivity. reflexivity. symmetry. apply Eempty. apply Em. apply MTE.
-  - intros G1 G2 REC idB B Bel EQ2 G' A WF2 WF0. rewrite Aadd in EQ2. apply Below_nIn in Bel as NIN.
-    assert (BidB: B.(blk_id) = idB). {
-      apply WF2. eapply MapsTo_m. reflexivity. reflexivity. apply EQ2. now apply add_1.
-    } subst.
-    replace (elements G2) with ((B.(blk_id), B)::(elements G1)). 2: {
-      symmetry. apply eqlistA_eq. now apply elements_Add_Below.
-    } 
-    split. intros [H|H].
-    3: case (eq_dec A.(blk_id) B.(blk_id)); unfold eq ; [intros EQ|intros NEQ]; intros [MT2 RM0 WF'].
-    * apply pair_equal_spec in H as []. subst A G'. 
-      repeat split; trivial.
-      + eapply MapsTo_m. reflexivity. reflexivity. apply EQ2. now apply add_1.
-      + now apply remove_wf_map_cfg.
-    * apply REC in H as [HM1 HR0 WF']; trivial.
-      assert (NEQ: ~ A.(blk_id)===B.(blk_id)). { 
-        intro. apply NIN. exists A. eapply MapsTo_m. 4: apply HM1. now symmetry. reflexivity. reflexivity.
-      }
-      repeat split;trivial.
-      + eapply MapsTo_m. reflexivity. reflexivity. apply EQ2. apply add_2. now symmetry. trivial.
-      + eapply add_wf_map_cfg. apply NIN. eapply wf_map_cfg_eq. apply EQ2. trivial.
-    * assert (Heq: A=B). { 
-      eapply wf_map_cfg_blk. apply WF2. apply MT2. eapply MapsTo_m.
-      apply EQ. reflexivity. apply EQ2. now apply add_1.
-    } subst. now left.
-    * right. apply REC; trivial. eapply add_wf_map_cfg. apply NIN. eapply wf_map_cfg_eq. apply EQ2. trivial.
-      repeat split; trivial.
-      eapply add_3. symmetry. apply NEQ. eapply MapsTo_m.
-      reflexivity. reflexivity. symmetry. apply EQ2. trivial.
+  apply map_ind.
+  - split. set_solver. intros []. inversion IN0.
+  - unfold blocks_aux_P. intros id b G NIN IH G0 G' id' b'. rewrite map_to_list_insert; trivial; cbn. split.
+    * intros IN.
+      apply elem_of_cons in IN as [EQ|IN];
+        [apply pair_equal_spec in EQ as [H EQ]; apply pair_equal_spec in H as [-> ->]|apply IH in IN as []];
+        split; trivial; now simplify_map_eq.
+    * intros [EQ IN]. case (decide (id=id')); intros DEC; apply elem_of_cons; [left|right].
+      + subst. pose proof lookup_insert_rev _ _ _ _ IN. now subst.
+      + apply IH. split; trivial; now simplify_map_eq.
 Qed.
 
-Lemma blocks_correct: forall G G' b, wf_map_cfg G -> ((b, G') ∈ (blocks G) <-> blocks_sem G G' b).
+Lemma blocks_correct: forall G G' id b, (id, b, G') ∈ blocks G <-> blocks_sem G G' id b.
 Proof.
   intros. now apply blocks_aux_correct.
 Qed.
