theories/Branch.v
@@ -1,68 +1,56 @@
-From Vellvm Require Import Syntax ScopeTheory Semantics.
-From ITree Require Import ITree Eq.
-Require Import FSets.FMapAVL FSets.FMapFacts.
+From Vellvm Require Import Syntax Tactics.
+(* From ITree Require Import ITree Eq.
+Require Import FSets.FMapAVL FSets.FMapFacts. *)
 Require Import List.
-Import ListNotations.
-From Pattern Require Import IdModule MapCFG.
-Import Map MapF MapF.P MapF.P.F.
-Import IdOT MapCFG.
+(* Import ListNotations. *)
+From Pattern Require Import Base.
+Import gmap.
+(* Import Map MapF MapF.P MapF.P.F.
+Import IdOT MapCFG. *)
 
-Definition branches_aux (G: map_cfg) id b acc : list (blk*bid*bid*map_cfg) := match b.(blk_term) with
-  | TERM_Br _ l r => (b, l, r, (remove id G))::acc
+Definition branches_aux (G: ocfg) id b acc : list (bid*blk*ocfg) := match b.(blk_term) with
+  | TERM_Br _ l r => (id, b, (delete id G))::acc
   | _ => acc
 end.
 
-Definition branches (G: map_cfg): list (blk*bid*bid*map_cfg) := fold (branches_aux G) G [].
+Definition branches (G: ocfg): list (bid*blk*ocfg) := map_fold (branches_aux G) [] G.
 
-Record branch_aux_sem (G0 G G': map_cfg) (B: blk) l r := {
-  EQ: G' = (remove_id B G0);
-  BR: exists e, B.(blk_term) = TERM_Br e l r;
-  MT: MapsTo_id B G
+Record branch_aux_sem (G0 G G': ocfg) id b := {
+  EQ: G' = delete id G0;
+  BR: exists e l r, b.(blk_term) = TERM_Br e l r;
+  IN: G !! id = Some b
 }.
 
-Definition branch_sem G G' B l r := branch_aux_sem G G G' B l r.
+Definition branch_sem G G' id b := branch_aux_sem G G G' id b.
+
+Definition branches_aux_P G0 (s:list (bid*blk*ocfg)) G :=
+  forall id b G', (id, b, G') ∈ s <-> branch_aux_sem G0 G G' id b.
 
 Lemma branches_aux_correct:
-  forall G0 G G' b l r, wf_map_cfg G ->
-  (b, l , r, G') ∈ (fold (branches_aux G0) G []) <-> branch_aux_sem G0 G G' b l r.
+  forall G G0,
+  branches_aux_P G0 (map_fold (branches_aux G0) [] G) G.
 Proof.
-  intros G0 G. apply fold_rec_bis.
-  - intros * EQ REC * WF'. assert (WF: wf_map_cfg m) by now apply (wf_map_cfg_eq m'). split.
-    * intros IN.
-      apply REC in IN as [EQ' [e TERM] MT]; trivial. repeat split; trivial.
-      now exists e. eapply MapsTo_m. 4: apply MT. reflexivity. trivial. now symmetry.
-    * intros [EQ' [e TERM] MT]. apply REC; trivial. repeat split; trivial. now exists e.
-      eapply MapsTo_m. 4: apply MT. all: auto. reflexivity.
-  - intros * WF. split. intro H. destruct H.
-    intros [EQ' [e TERM] MT]. now apply empty_mapsto_iff in MT.
-  - intros idB B * MT NIN REC * WFa.
-    assert (H: B.(blk_id) = idB). { apply WFa. now apply add_1. }
-    assert (WF': wf_map_cfg m'). { eapply add_wf_map_cfg. apply NIN. apply WFa. }
-    subst. split. 
-    * unfold branches_aux. intros IN. remember B.(blk_term) as T. induction T.
-      3: destruct IN as [EQ|IN].
+  intros *. apply map_fold_ind; clear G; unfold branches_aux_P.
+  - split. intro H. inversion H. intros []. set_solver.
+  - intros id b G acc NIN IH id' b' G'. unfold branches_aux. split.
+    * intro IN. break_match_hyp. 3: apply elem_of_cons in IN as [EQ|IN].
       3: {
-        apply pair_equal_spec in EQ as [EQ EQG].
-        apply pair_equal_spec in EQ as [EQ EQ1].
-        apply pair_equal_spec in EQ as [EQ EQ2]. subst.
-        repeat split; trivial. exists v. now rewrite HeqT.
-        now apply add_1. 
+        repeat apply pair_equal_spec in EQ as [EQ ?]. subst.
+        split; trivial. now exists v, br1, br2. now simplify_map_eq.
       }
-      all: apply REC in IN as [EQ' [e TERM] MT']; trivial.
-      all: repeat split; trivial; [now exists e|].
-      all: apply add_2; [|apply MT'].
-      all: intros EQ; apply NIN; exists b.
-      all: apply eq_eq in EQ; rewrite EQ; apply MT'.
-    * intros [EQ' [e TERM] MT']. apply add_mapsto_iff in MT' as [[EQid EQb]|[NEQ MT']].
-      + subst b. unfold branches_aux. rewrite TERM. subst. now left.
-      + unfold branches_aux. remember B.(blk_term) as T. induction T.
-        3: right.
-        all: apply REC; trivial. all: split; trivial; now exists e.
+      all: apply IH in IN as []; split; trivial; now simplify_map_eq.
+    * intros [EQ (e & l & r & BR) IN]. break_match_goal.
+      3: case (decide (id=id')); intros DEC; apply elem_of_cons; [left | right].
+      3: {
+        subst. pose proof lookup_insert_rev _ _ _ _ IN. subst. rewrite BR in Heqt. inversion Heqt. now subst.
+      }
+      all: assert (id <> id') by (auto; intro; subst; simplify_map_eq; rewrite BR in Heqt; discriminate).
+      all: apply IH; split; trivial; [now exists e, l, r|now simplify_map_eq].
 Qed.
 
 Lemma branches_correct:
-  forall G G' b l r, wf_map_cfg G ->
-  (b,l,r,G') ∈ (branches G) <-> branch_sem G G' b l r.
+  forall G G' id b, 
+  (id,b,G') ∈ (branches G) <-> branch_sem G G' id b.
 Proof.
   intros. now apply branches_aux_correct.
 Qed.
