theories/Focus.v
@@ -1,25 +1,30 @@
-From Vellvm Require Import Syntax ScopeTheory Semantics.
-From ITree Require Import ITree Eq.
-Require Import FSets.FMapAVL FSets.FMapFacts.
+From Vellvm Require Import Syntax.
+(* From ITree Require Import ITree Eq.
+Require Import FSets.FMapAVL FSets.FMapFacts. *)
 Require Import List.
-Import ListNotations.
-From Pattern Require Import IdModule MapCFG.
-Import Map MapF MapF.P MapF.P.F.
-Import IdOT MapCFG.
+(* Import ListNotations. *)
+From Pattern Require Import Base.
+(* Import Map MapF MapF.P MapF.P.F.
+Import IdOT MapCFG. *)
+Import gmap.
 
-Fixpoint focus_rec l (g1 g2: map_cfg) :=
+Fixpoint focus_rec l (g1 g2: ocfg) :=
   match l with
   | [] => [(g1, g2)]
-  | (id,b)::q => focus_rec q g1 g2 ++ focus_rec q (remove id g1) (add id b g2)
+  | (id,b)::q => focus_rec q g1 g2 ++ focus_rec q (delete id g1) (<[id:=b]> g2)
 end.
 
-Definition focus (G: map_cfg) := focus_rec (elements G) G empty.
+Definition focus (G: ocfg) := focus_rec (map_to_list G) G ∅.
 
-Record focus_sem (G G1 G2: map_cfg): Prop := {
-  PART: Partition G G1 G2; 
-  WF1: wf_map_cfg G1;
-  WF2: wf_map_cfg G2
+Record focus_sem (G G1 G2: ocfg): Prop := {
+  SUB1: G1 ⊆ G;
+  SUB2: G2 ⊆ G;
+  PART: G1 ##ₘ G2;
+  CUP: G1 ∪ G2 = G
 }.
 
-Lemma focus_correct: forall G G1 G2, wf_map_cfg G -> ((G1, G2) ∈ (focus G)) <-> focus_sem G G1 G2.
+Definition focus_correct_P G := forall G1 G2, ((G1, G2) ∈ (focus G)) <-> focus_sem G G1 G2.
+
+Lemma focus_correct: forall G, forall G1 G2, ((G1, G2) ∈ (focus G)) <-> focus_sem G G1 G2.
+Proof.
 Admitted.
