theories/Head.v
@@ -2,100 +2,54 @@
     and proves the correctness and completeness of that function.
     It also provides a [predecessors] function and lemmas to reason on it. *)
 
-From Vellvm Require Import Syntax ScopeTheory Semantics.
-From ITree Require Import ITree Eq.
-Require Import FSets.FMapAVL FSets.FMapFacts.
+From Vellvm Require Import Syntax.
+From Pattern Require Import Base.
 Require Import List.
-Import ListNotations.
-From Pattern Require Import IdModule MapCFG.
-Import Map MapF MapF.P MapF.P.F.
-Import IdOT MapCFG.
+Import gmap.
 
-(** * This section defines the [predecessors] and [heads] functions and their semantic. *)
+Definition is_empty (S: gset bid) := decide (S = ∅).
 
-Definition predecessors_aux (b id: bid) (bk: blk) := is_predecessor b bk.
-
-Definition predecessors (b : bid) (G : map_cfg) : map_cfg :=
-    filter (predecessors_aux b) G.
-
-Definition heads_aux (G: map_cfg) id b acc : list (blk*map_cfg) :=
+Definition heads_aux (G: ocfg) id b acc : list (bid*blk*ocfg) :=
   if is_empty (predecessors id G)
-  then (b, remove id G)::acc
+  then (id, b, delete id G)::acc
   else acc.
 
-Definition heads (G: map_cfg): list (blk*map_cfg) := fold (heads_aux G) G [].
+Definition heads (G: ocfg): list (bid*blk*ocfg) := map_fold (heads_aux G) [] G.
 
-Record heads_aux_sem (G0 G G': map_cfg) b := {
-  EQ: G' = (remove_id b G0);
-  WF: wf_map_cfg G';
-  MT: MapsTo_id b G;
-  PRED: Empty (predecessors b.(blk_id) G0)
+Record heads_aux_sem (G0 G G': ocfg) id b := {
+  EQ: G' = delete id G0;
+  IN: G !! id = Some b;
+  PRED: predecessors id G0 = ∅
 }.
 
-Definition heads_sem (G G':map_cfg) (b:blk) := heads_aux_sem G G G' b.
+Definition heads_sem (G G':ocfg) (id:bid) b := heads_aux_sem G G G' id b.
 
 (** * This section contains lemmas used for the proof of corectness and completeness of [Head]'s semantics. *)
 
-Lemma heads_aux_sem_eq: forall G0 G G' G1 b, G' ≡ G -> heads_aux_sem G0 G G1 b <-> heads_aux_sem G0 G' G1 b.
-Proof.
-  intros GO G G' G1 b EQIV. assert (EQIV': G ≡ G') by now symmetry.
-  split; intros [EQ WF MT PRED]; repeat split; trivial;
-  eapply MapsTo_m; try apply EQIV; try apply EQIV'; try reflexivity; trivial.
-Qed.
-
-Lemma heads_aux_split: forall A B id acc G G',
-  (A, G) ∈ (heads_aux G' id B acc) -> Empty (predecessors id G') /\ A = B /\ G = remove id G' \/ (A, G) ∈ acc.
-Proof.
-  unfold heads_aux. intros A B id acc G G'.
-  remember (is_empty (predecessors id G')) as b. induction b; [intros [EQ|IN]|intros IN].
-  left. apply pair_equal_spec in EQ as [ ]. rewrite is_empty_iff. now subst.
-  all: now right.
-Qed.
-
 (** The proof of corectness and completeness of [Head]'s semantics. *)
 
+Definition heads_aux_P G0 (s:list (bid*blk*ocfg)) G := forall id b G', (id, b, G') ∈ s <-> heads_aux_sem G0 G G' id b.
+
 Lemma heads_aux_correct:
-  forall G G0 G' b, wf_map_cfg G -> wf_map_cfg G0 ->
-  (b, G') ∈ (fold (heads_aux G0) G []) <-> heads_aux_sem G0 G G' b.
+  forall G G0,
+  heads_aux_P G0 (map_fold (heads_aux G0) [] G) G.
 Proof.
-  intros G G0. apply fold_rec_bis.
-  - intros G1 G2 acc EQ REC. intros. setoid_rewrite heads_aux_sem_eq. 2:apply EQ.
-    apply REC; [apply (wf_map_cfg_eq G2)|];trivial. now symmetry.
-  - intros. split. try contradiction. intros [_ _ MT _].
-    now apply empty_mapsto_iff in MT.
-  - intros idB B acc G1 MTB NIN REC G2 A WF WF0.
-    assert (HidB: B.(blk_id) = idB). { apply WF. now apply add_1. } subst idB.
-    split.
-    * intros H. apply heads_aux_split in H as [[EM [EQA EQG]]|IN].
-      + subst. split; trivial.
-        -- now apply remove_wf_map_cfg.
-        -- now apply add_1.
-      + assert (H: (heads_aux_sem G0 G1 G2 A)). { 
-          apply REC; trivial.
-          eapply wf_map_cfg_eq. 2: { apply remove_wf_map_cfg. apply WF. }
-          symmetry. now apply remove_add_elim.
-        } destruct H as [EQ WF2 MTA PRED]. split; trivial.
-        case (eq_dec A.(blk_id) B.(blk_id)); unfold eq; [intros EQID|intros NEQID].
-        -- contradict NIN. exists A. apply eq_eq in EQID. now rewrite <- EQID.
-        -- eapply add_2. now symmetry. trivial.
-    * intros [EQ WF2 MTA PRED]. unfold heads_aux.
-      (case (eq_dec A.(blk_id) B.(blk_id)); unfold eq; [intros EQID|intros NEQID]).
-      + assert (H: A=B). {
-            eapply MapsTo_fun. apply MTA. apply eq_eq in EQID. rewrite EQID. now apply add_1.
-          } subst. remember (is_empty (predecessors B.(blk_id) G0)) as b. induction b.
-        -- now left.
-        -- apply is_empty_iff in PRED. rewrite PRED in Heqb. discriminate.
-      + assert (H: (A, G2) ∈ acc). {
-          apply REC. eapply add_wf_map_cfg. apply NIN. apply WF. trivial.
-          repeat split; trivial. eapply add_3. symmetry. apply NEQID. apply MTA.
-        } remember (is_empty (predecessors B.(blk_id) G0)) as b. induction b.
-        -- now right.
-        -- trivial.
+  intros *. apply map_fold_ind; clear G.
+  - unfold heads_aux_P. split; intro H; inversion H. set_solver.
+  - unfold heads_aux_P. intros id b G r NIN IH id' b' G'. split.
+    * unfold heads_aux. case (is_empty (predecessors id G0)); intros EM IN.
+      apply elem_of_cons in IN as [EQ|IN]. apply pair_equal_spec in EQ as [H EQ]. apply pair_equal_spec in H as [-> ->].
+      2, 3: apply IH in IN as [EQ IN PRED]. all: split; trivial; now simplify_map_eq.
+    * unfold heads_aux. intros [EQ IN PRED].
+      case (is_empty (predecessors id G0)); intros EM. case (decide (id=id')); intros DEC; apply elem_of_cons; [left | right].
+      subst. pose proof lookup_insert_rev _ _ _ _ IN. now subst.
+      2: assert (id <> id') by (intro; now subst).
+      all: apply IH; split; trivial; now simplify_map_eq.
 Qed.
 
 Lemma heads_correct:
-  forall G G' b, wf_map_cfg G ->
-  (b, G') ∈ (heads G) <-> heads_sem G G' b.
+  forall G G' id b,
+  (id, b, G') ∈ (heads G) <-> heads_sem G G' id b.
 Proof.
   intros. now apply heads_aux_correct.
 Qed.
@@ -103,7 +57,7 @@ Qed.
 (** * This section contains lemmas used to manipulate [predecessors] on a remove,
       e.g. for the proofs of [BlockFusion]. *)
 
-Lemma Proper_predecessor_aux:
+(* Lemma Proper_predecessor_aux:
   forall id, Proper (eq' ==> Logic.eq ==> Logic.eq) (predecessors_aux id).
 Proof.
   now intro.
@@ -145,4 +99,4 @@ Proof.
       apply MTC. contradict MTC. intros MTC. eapply remove_mapsto_iff. apply MTC. now subst.
     * eapply add_3. apply NEQ. apply PRED. split; trivial. eapply remove_3. apply MTC.
   - intro MTC. contradict MTC. intro MTC. eapply empty_mapsto_iff. apply MTC.
-Qed.
+Qed. *)
