theories/Patterns.v
@@ -1,24 +1,25 @@
 (** This file defines [Pattern]s, the [MatchAll] function to interpret them, and correctness proofs. *)
 
-From Vellvm Require Import Syntax ScopeTheory Semantics.
-From ITree Require Import ITree Eq.
-From Pattern Require Import IdModule MapCFG Head Focus Block Branch.
-Require Import FSets.FMapAVL FSets.FMapFacts.
+From Vellvm Require Import Syntax.
+(* From ITree Require Import ITree Eq. *)
+From Pattern Require Import Base Head Focus Block Branch.
+(* Require Import FSets.FMapAVL FSets.FMapFacts. *)
 Require Import List.
-Import ListNotations.
-Import Map MapF MapF.P MapF.P.F.
-Import IdOT MapCFG Head Focus Block Branch.
+(* Import ListNotations. *)
+Import gmap.
+(* Import Map MapF MapF.P MapF.P.F.
+Import IdOT MapCFG Head Focus Block Branch. *)
 
 (** This section defines the [Pattern] type and the [MatchAll] function to interpret them. *)
 
 Inductive Pattern : Type -> Type :=
-  | Graph: Pattern map_cfg
+  | Graph: Pattern ocfg
   | When: forall {S}, Pattern S -> (S -> bool) -> Pattern S
-  | Head: forall {S}, Pattern S -> Pattern (blk * S)
-  | Focus: forall {S}, Pattern S -> Pattern (map_cfg * S)
+  | Head: forall {S}, Pattern S -> Pattern (bid * blk * S)
+  | Focus: forall {S}, Pattern S -> Pattern (ocfg * S)
   | Map: forall {S} {T}, Pattern S -> (S -> T) -> Pattern T
-  | Block: forall {S}, Pattern S -> Pattern (blk * S)
-  | Branch: forall {S}, Pattern S -> Pattern (blk * bid * bid * S)
+  | Block: forall {S}, Pattern S -> Pattern (bid * blk * S)
+  | Branch: forall {S}, Pattern S -> Pattern (bid * blk * S)
 .
 
 Notation "□" := Graph.
@@ -28,16 +29,16 @@ Definition flat_map_r {A B C} (f : B -> list C) :=
   fix flat_map_r (l : list (A*B)) : list (A*C) :=
     match l with
     | [] => []
-    | (a, b)::q => List.map (fun c => (a, c)) (f b)++flat_map_r q
+    | (a, b)::q => ((fun c => (a, c)) <$> (f b))++flat_map_r q
 end.
 
-Fixpoint MatchAll {S} (P: Pattern S) (g: map_cfg) : list S :=
+Fixpoint MatchAll {S} (P: Pattern S) (g: ocfg) : list S :=
   match P with
     | □ => [g]
     | Head _ p => flat_map_r (MatchAll p) (heads g)
     | Focus _ p => flat_map_r (MatchAll p) (focus g)
-    | p when f => List.filter f (MatchAll p g) 
-    | Map _ _ p f => List.map f (MatchAll p g)
+    | p when f => filter (fun x => f x = true) (MatchAll p g) 
+    | Map _ _ p f => f <$> (MatchAll p g)
     | Block _ p => flat_map_r (MatchAll p) (blocks g)
     | Branch _ p => flat_map_r (MatchAll p) (branches g)
 end.
@@ -53,68 +54,65 @@ Lemma in_flat_map_r {A B C}:
   exists b, (a,b) ∈ l /\ c ∈ (f b).
 Proof.
   intro f. induction l as [|[a b] l IHl].
-  * intros. split. contradiction. intros [b [H1 H2]]. contradiction.
+  * intros. cbn. split. intro H. inversion H. intros [b [H1 H2]]. inversion H1.
   * intros a' c'. split.
-    - cbn. intro IN. apply in_app_or in IN as [IN|IN].
-      + exists b.
-        apply Coqlib.list_in_map_inv in IN as [c'' [EQ IN]].
+    - cbn. intro IN. apply elem_of_app in IN as [IN|IN].
+      + exists b. apply elem_of_list_fmap in IN as [c'' [EQ IN]].
         apply pair_equal_spec in EQ as []. subst.
-        split; trivial. left. apply pair_equal_spec. now split.
-      + assert (H': exists b0 : B, (a', b0) ∈ l /\ c' ∈ (f b0)) by now apply IHl.
-        destruct H' as [b' [IN1 IN2]]. exists b'. split; trivial. now right.
-    - intros [b' [[EQ|IN1] IN2]];cbn; apply in_or_app.
-      + apply pair_equal_spec in EQ as []. subst. left. now apply in_map.
-      + right. apply IHl. now exists b'. 
+        split; trivial. left.
+      + assert (exists b0 : B, (a', b0) ∈ l /\ c' ∈ (f b0)) as [b' [IN1 IN2]] by now apply IHl.
+        exists b'. split; trivial. now right.
+    - intros [b' [IN1 IN2]]. apply elem_of_cons in IN1 as [EQ|IN1]; cbn; apply elem_of_app; [left|right].
+      + apply pair_equal_spec in EQ as []. subst. apply elem_of_list_fmap. now exists c'.
+      + apply IHl. now exists b'. 
 Qed.
 
 Theorem Pattern_Graph_correct: forall G G', G' ∈ (MatchAll □ G) -> G' = G.
 Proof.
-  cbn. intros G G' H. destruct H; now destruct H.
+  cbn. intros G G' H. set_solver.
 Qed.
 
 Theorem Pattern_Head_correct {S}:
-  forall (G: map_cfg) (P: Pattern S) (b:blk) X, wf_map_cfg G ->
-  (b, X) ∈ (MatchAll (Head P) G) <->
-  exists G', heads_sem G G' b /\ X ∈ (MatchAll P G').
+  forall (G: ocfg) (P: Pattern S) id b X,
+  (id, b, X) ∈ (MatchAll (Head P) G) <->
+  exists G', heads_sem G G' id b /\ X ∈ (MatchAll P G').
 Proof.
-  intros G P b X WF. setoid_rewrite <- heads_correct;trivial. apply in_flat_map_r.
+  intros *. setoid_rewrite <- heads_correct;trivial. apply in_flat_map_r.
 Qed.
 
 Theorem Pattern_Focus_correct {S}:
-  forall (G G1: map_cfg) (P:Pattern S) X, wf_map_cfg G ->
+  forall (G G1: ocfg) (P:Pattern S) X, 
   (G1, X) ∈ (MatchAll (Focus P) G) <-> exists G2, focus_sem G G1 G2 /\ X ∈ (MatchAll P G2).
 Proof.
-  intros G G1 P X WF. setoid_rewrite <-focus_correct;trivial. apply in_flat_map_r.
+  intros *. setoid_rewrite <-focus_correct;trivial. apply in_flat_map_r.
 Qed.
 
 Theorem Pattern_When_correct {S}:
   forall (P: Pattern S) f X G,
-  X ∈ (MatchAll (P when f) G) <-> X ∈ (MatchAll P G) /\ f X = true.
+  X ∈ (MatchAll (P when f) G) <-> f X = true /\ X ∈ (MatchAll P G).
 Proof.
-  intros. apply filter_In.
+  intros. cbn. now rewrite elem_of_list_filter.
 Qed.
 
 Theorem Pattern_Map_correct {S T}:
   forall (P: Pattern S) (f: S -> T) X G,
-  X ∈ (MatchAll (Map P f) G) <-> exists y, f y = X /\ y ∈ (MatchAll P G).
+  X ∈ (MatchAll (Map P f) G) <-> exists y, X = f y /\ y ∈ (MatchAll P G).
 Proof.
-  cbn. intros P f X G. split.
-  - intro H. apply Coqlib.list_in_map_inv in H as [y [H1 H2]]. now exists y.
-  - intros [y [H1 H2]]. subst. now apply in_map.
+  cbn. intros P f X G. now rewrite elem_of_list_fmap.
 Qed.
 
 Theorem Pattern_Block_correct {S}:
-  forall (G: map_cfg) (P: Pattern S) (b:blk) X, wf_map_cfg G ->
-  (b, X) ∈ (MatchAll (Block P) G) <->
-  exists G', blocks_sem G G' b /\ X ∈ (MatchAll P G').
+  forall (G: ocfg) (P: Pattern S) id (b:blk) X,
+  (id, b, X) ∈ (MatchAll (Block P) G) <->
+  exists G', blocks_sem G G' id b /\ X ∈ (MatchAll P G').
 Proof.
   intros. setoid_rewrite <-blocks_correct;trivial. apply in_flat_map_r.
 Qed.
 
 Theorem Pattern_Branch_correct {S}:
-  forall G P B l r (s:S), wf_map_cfg G ->
-  (B,l,r,s) ∈ (MatchAll (Branch P) G) <->
-  exists G', branch_sem G G' B l r /\ s ∈ (MatchAll P G').
+  forall G P B id (s:S),
+  (id,B,s) ∈ (MatchAll (Branch P) G) <->
+  exists G', branch_sem G G' id B /\ s ∈ (MatchAll P G').
 Proof.
   intros. setoid_rewrite <-branches_correct; trivial. apply in_flat_map_r.
 Qed.
